formal-proofs/theories/lib/concurrent_linked_list/list_interfaces.v
@@ -1,0 +1,10 @@
+From iris.heap_lang Require Export notation.
+
+Record listInterface :=
+  ListInterface {
+      newList: val;
+      cleanPrev: val;
+      findSegment: val;
+      moveForward: val;
+      onSlotCleaned: val;
+    }.
